Logic/Predicate/Semantics.lean
@@ -6,63 +6,76 @@ variable
   {L : Language.{u}} {L₁ : Language.{u₁}} {L₂ : Language.{u₂}}
   {μ : Type v} {μ₁ : Type v₁} {μ₂ : Type v₂}
 
-@[ext] class Structure₁ (L : Language.{u}) (M : Type w) where
+namespace FirstOrder
+
+@[ext] class Structure (L : Language.{u}) (M : Type w) where
   func : {k : ℕ} → L.func k → (Fin k → M) → M
   rel  : {k : ℕ} → L.rel k → (Fin k → M) → Prop
 
+end FirstOrder
+
 namespace Language
+
 namespace Hom
 
-def onStructure₁ (Φ : L₁ →ᵥ L₂) {M : Type w} (S : Structure₁ L₂ M) : Structure₁ L₁ M where
+open FirstOrder
+
+def onStructure (Φ : L₁ →ᵥ L₂) {M : Type w} (S : Structure L₂ M) : Structure L₁ M where
   func := fun f => S.func (Φ.onFunc f)
   rel := fun r => S.rel (Φ.onRel r)
 
-instance subLanguageStructure₁ {pf : ∀ k, Language.func L k → Prop} {pr : ∀ k, L.rel k → Prop}
-  {M : Type w} (s : Structure₁ L M) : Structure₁ (subLanguage L pf pr) M :=
-  onStructure₁ (ofSubLanguage L) s
+instance subLanguageStructure {pf : ∀ k, Language.func L k → Prop} {pr : ∀ k, L.rel k → Prop}
+  {M : Type w} (s : Structure L M) : Structure (subLanguage L pf pr) M :=
+  onStructure (ofSubLanguage L) s
 
-noncomputable def extendStructure₁ (Φ : L₁ →ᵥ L₂) {M : Type w} [Inhabited M] (s : Structure₁ L₁ M) : Structure₁ L₂ M where
+noncomputable def extendStructure (Φ : L₁ →ᵥ L₂) {M : Type w} [Inhabited M] (s : Structure L₁ M) : Structure L₂ M where
   func := fun {k} f₂ v => Classical.epsilon (fun y => ∃ f₁ : L₁.func k, Φ.onFunc f₁ = f₂ ∧ y = s.func f₁ v)
   rel  := fun {k} r₂ v => ∃ r₁ : L₁.rel k, Φ.onRel r₁ = r₂ ∧ s.rel r₁ v
 
 end Hom
 end Language
 
-namespace Structure₁
+namespace FirstOrder
 
-instance [Inhabited M] : Inhabited (Structure₁ L M) :=
+namespace Structure
+
+instance [Inhabited M] : Inhabited (Structure L M) :=
 ⟨{ func := fun _ _ => default, rel := fun _ _ => True }⟩
 
-variable (Φ : L₁ →ᵥ L₂) {M : Type w} (s₂ : Structure₁ L₂ M)
+variable (Φ : L₁ →ᵥ L₂) {M : Type w} (s₂ : Structure L₂ M)
 
-@[simp] lemma onStructure₁_func {k} {f : L₁.func k} {v : Fin k → M} :
-    (Φ.onStructure₁ s₂).func f v = s₂.func (Φ.onFunc f) v := rfl
+@[simp] lemma onStructure_func {k} {f : L₁.func k} {v : Fin k → M} :
+    (Φ.onStructure s₂).func f v = s₂.func (Φ.onFunc f) v := rfl
 
-@[simp] lemma onStructure₁_rel {k} {r : L₁.rel k} {v : Fin k → M} :
-    (Φ.onStructure₁ s₂).rel r v ↔ s₂.rel (Φ.onRel r) v := of_eq rfl
+@[simp] lemma onStructure_rel {k} {r : L₁.rel k} {v : Fin k → M} :
+    (Φ.onStructure s₂).rel r v ↔ s₂.rel (Φ.onRel r) v := of_eq rfl
 
-variable [Inhabited M] (s₁ : Structure₁ L₁ M)
+variable [Inhabited M] (s₁ : Structure L₁ M)
 
-lemma extendStructure₁_func
+lemma extendStructure_func
   {k} (injf : Function.Injective (Φ.onFunc : L₁.func k → L₂.func k)) (f₁ : L₁.func k) (v : Fin k → M) :
-    (Φ.extendStructure₁ s₁).func (Φ.onFunc f₁) v = s₁.func f₁ v := by
-  simp[Language.Hom.extendStructure₁]
+    (Φ.extendStructure s₁).func (Φ.onFunc f₁) v = s₁.func f₁ v := by
+  simp[Language.Hom.extendStructure]
   have : ∃ y, ∃ f₁' : L₁.func k, Φ.onFunc f₁' = Φ.onFunc f₁ ∧ y = s₁.func f₁' v := ⟨s₁.func f₁ v, f₁, rfl, rfl⟩
   rcases Classical.epsilon_spec this with ⟨f', f'eq, h⟩
   rcases injf f'eq with rfl; exact h
 
-lemma extendStructure₁_rel
+lemma extendStructure_rel
   {k} (injr : Function.Injective (Φ.onRel : L₁.rel k → L₂.rel k)) (r₁ : L₁.rel k) (v : Fin k → M) :
-    (Φ.extendStructure₁ s₁).rel (Φ.onRel r₁) v ↔ s₁.rel r₁ v := by
-  simp[Language.Hom.extendStructure₁]
+    (Φ.extendStructure s₁).rel (Φ.onRel r₁) v ↔ s₁.rel r₁ v := by
+  simp[Language.Hom.extendStructure]
   refine ⟨by intros h; rcases h with ⟨r₁', e, h⟩; rcases injr e; exact h, by intros h; refine ⟨r₁, rfl, h⟩⟩
 
 
-end Structure₁
+end Structure
+
+end FirstOrder
 
 namespace SubTerm
 
-variable {M} (s : Structure₁ L M) {n n₁ n₂ : ℕ} (e : Fin n → M) (e₂ : Fin n₂ → M) (ε : μ → M) (ε₂ : μ₂ → M)
+open FirstOrder
+
+variable {M} (s : Structure L M) {n n₁ n₂ : ℕ} (e : Fin n → M) (e₂ : Fin n₂ → M) (ε : μ → M) (ε₂ : μ₂ → M)
 
 def val : SubTerm L μ n → M
   | #x       => e x
@@ -71,7 +84,7 @@ def val : SubTerm L μ n → M
 
 variable (M) {s}
 
-@[reducible] def val! (M : Type w) [s : Structure₁ L M] {n} (e : Fin n → M) (ε : μ → M) : SubTerm L μ n → M := val s e ε
+@[reducible] def val! (M : Type w) [s : Structure L M] {n} (e : Fin n → M) (ε : μ → M) : SubTerm L μ n → M := val s e ε
 
 variable {M e e₂ ε ε₂}
 
@@ -97,21 +110,22 @@ lemma val_subst (u : SubTerm L μ n) (t : SubTerm L μ (n + 1)) :
     t.bShift.val s (a :> e) ε = t.val s e ε := by simp[bShift, val_map, Function.comp]
 
 section Language
+
 variable (Φ : L₁ →ᵥ L₂) (e : Fin n → M) (ε : μ → M)
 
-lemma val_onSubTerm (s₂ : Structure₁ L₂ M) {t : SubTerm L₁ μ n} :
-    val s₂ e ε (Φ.onSubTerm t) = val (Φ.onStructure₁ s₂) e ε t :=
+lemma val_onSubTerm (s₂ : Structure L₂ M) {t : SubTerm L₁ μ n} :
+    val s₂ e ε (Φ.onSubTerm t) = val (Φ.onStructure s₂) e ε t :=
   by induction t <;> simp[*, val!, Function.comp, val_func, Language.Hom.onSubTerm_func]
 
 variable [Inhabited M]
 
-lemma val_extendStructure₁_onSubTerm
+lemma val_extendStructure_onSubTerm
     (injf : ∀ k, Function.Injective (Φ.onFunc : L₁.func k → L₂.func k))
-    (s₁ : Structure₁ L₁ M) (t : SubTerm L₁ μ n) :
-    val (Φ.extendStructure₁ s₁) e ε (Φ.onSubTerm t) = val s₁ e ε t := by
+    (s₁ : Structure L₁ M) (t : SubTerm L₁ μ n) :
+    val (Φ.extendStructure s₁) e ε (Φ.onSubTerm t) = val s₁ e ε t := by
   induction t <;> simp[*, Language.Hom.onSubTerm_func, val_func]
   case func k f v ih => 
-    exact Structure₁.extendStructure₁_func Φ s₁ (injf k) f (fun i => val s₁ e ε (v i))
+    exact Structure.extendStructure_func Φ s₁ (injf k) f (fun i => val s₁ e ε (v i))
 
 end Language
 
